Refactor program.v

theories/program/Program.v
@@ -14,7 +14,7 @@ Section PROGRAM.
 
 Variable nq : nat. (* number of qubits *)
 
-(* inlined QASM instructions ================================================================= *)
+(* desugared QASM instructions ================================================================== *)
 
 Inductive Instruction: Type :=
 | NopInstr: Instruction
@@ -28,7 +28,7 @@ Inductive Instruction: Type :=
 
 
 (* ============================================================================================== *)
-(* inlined QASM program ====================================================================== *)
+(* desugared QASM program ======================================================================= *)
 
 Record InlinedProgram: Type := {
   IP_num_cbits: nat;
@@ -37,85 +37,85 @@ Record InlinedProgram: Type := {
 }.
 
 (* ============================================================================================== *)
-(* MWI for program states ======================================================================= *)
+(* Branching for program states ================================================================= *)
 
-Record World: Type := {
-  W_num_clbits: nat;
-  W_qstate: Matrix nq; (* density matrix *)
-  W_cstate: total_map bool;  (* false for 0, true for 1 *)
-  W_prob: R; (* probability of the world *)
-  W_prob_valid: (W_prob > 0)%R;
+Record Branch: Type := {
+  B_num_clbits: nat;
+  B_qstate: Matrix nq; (* density matrix *)
+  B_cstate: total_map bool;  (* false for 0, true for 1 *)
+  B_prob: R; (* probability of the branch *)
+  B_prob_valid: (B_prob > 0)%R;
 }.
 
-Definition qstate_valid (w: World): Prop := den_valid (W_qstate w).
+Definition qstate_valid (b: Branch): Prop := den_valid (B_qstate b).
 
 (* ============================================================================================== *)
-(* ManyWorlds for program states =============================================================== *)
+(* Program state ================================================================================ *)
 
-Definition ManyWorld: Type := list World.
+Definition ProgramState: Type := list Branch.
 
-Definition ManyWorld_init (num_q num_c: nat): ManyWorld.
+Definition ProgramState_init (num_q num_c: nat): ProgramState.
 Proof.
   refine ([{|
-    W_num_clbits := num_c;
-    W_qstate := den_init nq;
-    W_cstate := tm_empty false;
-    W_prob := 1;
+    B_num_clbits := num_c;
+    B_qstate := den_init nq;
+    B_cstate := tm_empty false;
+    B_prob := 1;
   |}]).
   lra.
 Defined.
 
 (* ============================================================================================== *)
-(* merging two worlds =========================================================================== *)
+(* merging two branches =========================================================================== *)
 
-Definition Merge_world (w0 w1: World): World.
+Definition Merge_branch (b0 b1: Branch): Branch.
 Proof.
-  destruct w0 eqn:ew0, w1.
+  destruct b0 eqn:ew0, b1.
   destruct
-    (Nat.eq_dec W_num_clbits0 W_num_clbits1),
-    (tmb_equal W_cstate0 W_cstate1 W_num_clbits0) eqn:ec.
-  subst W_num_clbits1.
+    (Nat.eq_dec B_num_clbits0 B_num_clbits1),
+    (tmb_equal B_cstate0 B_cstate1 B_num_clbits0) eqn:ec.
+  subst B_num_clbits1.
   refine ({|
-    W_num_clbits := W_num_clbits0;
-    W_qstate := W_prob0 .* W_qstate0 + W_prob1 .* W_qstate1;
-    W_cstate := W_cstate0;
-    W_prob := W_prob0 + W_prob1;
+    B_num_clbits := B_num_clbits0;
+    B_qstate := B_prob0 .* B_qstate0 + B_prob1 .* B_qstate1;
+    B_cstate := B_cstate0;
+    B_prob := B_prob0 + B_prob1;
   |}).
   lra.
-  all: exact w0.
+  all: exact b0.
 Defined.
 
-Definition Merge_manyworld_suppl (w: World) (mw: ManyWorld): ManyWorld.
+Definition Merge_program_state_suppl (b: Branch) (ps: ProgramState): ProgramState.
 Proof.
-  induction mw.
-  - exact [w].
+  induction ps.
+  - exact [b].
   - destruct
-    (tmb_equal (W_cstate a) (W_cstate w) (W_num_clbits a)).
-    destruct w as [nc qst cst p pv], a as [nc' qst' cst' p' pv']; simpl in *.
+    (tmb_equal (B_cstate a) (B_cstate b) (B_num_clbits a)).
+    destruct b as [nc qst cst p pv], a as [nc' qst' cst' p' pv']; simpl in *.
     refine ({|
-      W_num_clbits := nc;
-      W_qstate := (p / (p + p'))%com .* qst + (p' / (p + p'))%com .* qst';
-      W_cstate := cst;
-      W_prob := p + p';
-    |} :: mw). (* merge *)
+      B_num_clbits := nc;
+      B_qstate := (p / (p + p'))%com .* qst + (p' / (p + p'))%com .* qst';
+      B_cstate := cst;
+      B_prob := p + p';
+    |} :: ps). (* merge *)
       lra.
-    exact (a :: IHmw). (* nop *)
+    exact (a :: IHps). (* nop *)
 Defined.
 
-Definition Merge_manyworld (mw: ManyWorld): ManyWorld.
+Definition Merge_program_state (ps: ProgramState): ProgramState.
 Proof.
-  destruct mw.
+  destruct ps.
   - exact [].
-  - destruct mw.
-    + exact (Merge_manyworld_suppl w []).
-    + exact (Merge_manyworld_suppl w (Merge_manyworld_suppl w0 mw)).
+  - destruct ps.
+    + exact (Merge_program_state_suppl b []).
+    + exact (Merge_program_state_suppl b (Merge_program_state_suppl b0 ps)).
 Defined.
 
-Lemma Merge_manyworld_suppl_qstate_valid:
-  forall (w: World) (mw: ManyWorld),
-  den_valid (W_qstate w) -> Forall qstate_valid mw -> Forall qstate_valid (Merge_manyworld_suppl w mw).
+Lemma Merge_program_state_suppl_qstate_valid:
+  forall (b: Branch) (ps: ProgramState),
+  den_valid (B_qstate b) -> Forall qstate_valid ps -> Forall qstate_valid (Merge_program_state_suppl b ps).
 Proof.
-  induction mw.
+  induction ps.
   - intros; simpl.
     apply Forall_cons.
     apply H.
@@ -123,8 +123,8 @@ Proof.
   - intros; simpl.
     apply Forall_cons_iff in H0.
     destruct H0.
-    destruct (tmb_equal (W_cstate a) (W_cstate w) (W_num_clbits a)).
-    + destruct w as [nc qst cst p pv], a as [nc' qst' cst' p' pv']; simpl in *.
+    destruct (tmb_equal (B_cstate a) (B_cstate b) (B_num_clbits a)).
+    + destruct b as [nc qst cst p pv], a as [nc' qst' cst' p' pv']; simpl in *.
       apply Forall_cons.
       * apply den_valid_mix.
         all: assumption.
@@ -132,122 +132,122 @@ Proof.
     + apply Forall_cons; auto; auto.
 Qed.
 
-Lemma Merge_manyworld_qstate_valid:
-  forall (worlds: ManyWorld),
-  Forall qstate_valid worlds -> Forall qstate_valid (Merge_manyworld worlds).
+Lemma Merge_program_state_qstate_valid:
+  forall (branches: ProgramState),
+  Forall qstate_valid branches -> Forall qstate_valid (Merge_program_state branches).
 Proof.
   intros; simpl.
-  induction worlds as [|w0[|w1 t] ].
+  induction branches as [|b0[|b1 t] ].
   - apply Forall_nil.
   - apply H.
   - apply Forall_cons_iff in H; destruct H.
     apply Forall_cons_iff in H0; destruct H0.
-    apply Merge_manyworld_suppl_qstate_valid.
+    apply Merge_program_state_suppl_qstate_valid.
     all: auto.
-    apply Merge_manyworld_suppl_qstate_valid.
+    apply Merge_program_state_suppl_qstate_valid.
     all: auto.
 Qed.
 
 (* ============================================================================================== *)
 (* execution ==================================================================================== *)
 
-Fixpoint Execute_rotate_instr (theta phi lambda: R) (target: nat) (worlds: ManyWorld): ManyWorld.
+Fixpoint Execute_rotate_instr (theta phi lambda: R) (target: nat) (branches: ProgramState): ProgramState.
 Proof.
-  destruct worlds as [|[nc qstate cstate prob Hp] t].
+  destruct branches as [|[nc qstate cstate prob Hp] t].
   - exact [].
   - destruct (lt_dec target nq).
     + exact ({|
-        W_num_clbits := nc;
-        W_qstate := den_uop (mat_single nq target (mat_rot theta phi lambda)) qstate ;
-        W_cstate := cstate;
-        W_prob := prob;
-        W_prob_valid := Hp;
+        B_num_clbits := nc;
+        B_qstate := den_uop (mat_single nq target (mat_rot theta phi lambda)) qstate ;
+        B_cstate := cstate;
+        B_prob := prob;
+        B_prob_valid := Hp;
       |} :: (Execute_rotate_instr theta phi lambda target t)).
     + exact ({|
-        W_num_clbits := nc;
-        W_qstate := qstate;
-        W_cstate := cstate;
-        W_prob := prob;
-        W_prob_valid := Hp;
+        B_num_clbits := nc;
+        B_qstate := qstate;
+        B_cstate := cstate;
+        B_prob := prob;
+        B_prob_valid := Hp;
       |} :: (Execute_rotate_instr theta phi lambda target t)).  (* nop *)
 Defined.
 
-Fixpoint Execute_cnot_instr (control target: nat) (worlds: ManyWorld): ManyWorld.
+Fixpoint Execute_cnot_instr (control target: nat) (branches: ProgramState): ProgramState.
 Proof.
-  destruct worlds as [|[nc qstate cstate prob Hp] t].
+  destruct branches as [|[nc qstate cstate prob Hp] t].
   - exact [].
   - destruct (ge_dec nq 2), (lt_dec control nq), (lt_dec target nq).
     exact ({|
-      W_num_clbits := nc;
-      W_qstate := den_uop (mat_cnot control target) qstate;
-      W_cstate := cstate;
-      W_prob := prob;
-      W_prob_valid := Hp;
+      B_num_clbits := nc;
+      B_qstate := den_uop (mat_cnot control target) qstate;
+      B_cstate := cstate;
+      B_prob := prob;
+      B_prob_valid := Hp;
       |} :: (Execute_cnot_instr control target t)).
     all: refine ({|
-      W_num_clbits := nc;
-      W_qstate := qstate;
-      W_cstate := cstate;
-      W_prob := prob;
-      W_prob_valid := Hp;
+      B_num_clbits := nc;
+      B_qstate := qstate;
+      B_cstate := cstate;
+      B_prob := prob;
+      B_prob_valid := Hp;
     |} :: (Execute_cnot_instr control target t)).  (* nop *)
 Defined.
 
-Fixpoint Execute_swap_instr (q1 q2: nat) (worlds: ManyWorld): ManyWorld.
+Fixpoint Execute_swap_instr (q1 q2: nat) (branches: ProgramState): ProgramState.
 Proof.
-  destruct worlds as [|[nc qstate cstate prob Hp] t].
+  destruct branches as [|[nc qstate cstate prob Hp] t].
   - exact [].
   - destruct (lt_dec q1 nq), (lt_dec q2 nq).
     exact ({|
-      W_num_clbits := nc;
-      W_qstate := den_uop (mat_swap q1 q2) qstate;
-      W_cstate := cstate;
-      W_prob := prob;
-      W_prob_valid := Hp;
+      B_num_clbits := nc;
+      B_qstate := den_uop (mat_swap q1 q2) qstate;
+      B_cstate := cstate;
+      B_prob := prob;
+      B_prob_valid := Hp;
       |} :: (Execute_swap_instr q1 q2 t)).
     all: exact ({|
-        W_num_clbits := nc;
-        W_qstate := qstate;
-        W_cstate := cstate;
-        W_prob := prob;
-        W_prob_valid := Hp;
+        B_num_clbits := nc;
+        B_qstate := qstate;
+        B_cstate := cstate;
+        B_prob := prob;
+        B_prob_valid := Hp;
       |} :: (Execute_swap_instr q1 q2 t)).  (* nop *)
 Defined.
 
-Fixpoint Execute_measure_instr (qbit cbit: nat) (worlds: ManyWorld): ManyWorld.
+Fixpoint Execute_measure_instr (qbit cbit: nat) (branches: ProgramState): ProgramState.
 Proof.
-  destruct worlds as [|[nc qstate cstate prob Hp] t].
+  destruct branches as [|[nc qstate cstate prob Hp] t].
   - exact [].
   - destruct (lt_dec qbit nq).
     + specialize (com_real (den_prob_0 qbit qstate)) as prob0.
       specialize (com_real (den_prob_1 qbit qstate)) as prob1.
       destruct (Rgt_dec prob0 0), (Rgt_dec prob1 0).
       * refine ({|
-          W_num_clbits := nc;
-          W_qstate := den_measure_0 qbit qstate;
-          W_cstate := tm_update cstate cbit false;
-          W_prob := prob * prob0;
+          B_num_clbits := nc;
+          B_qstate := den_measure_0 qbit qstate;
+          B_cstate := tm_update cstate cbit false;
+          B_prob := prob * prob0;
         |} :: {|
-          W_num_clbits := nc;
-          W_qstate := den_measure_1 qbit qstate;
-          W_cstate := tm_update cstate cbit true;
-          W_prob := prob * prob1;
+          B_num_clbits := nc;
+          B_qstate := den_measure_1 qbit qstate;
+          B_cstate := tm_update cstate cbit true;
+          B_prob := prob * prob1;
         |} ::
         (Execute_measure_instr qbit cbit t)).
         all: try nra.
       * refine ({|
-          W_num_clbits := nc;
-          W_qstate := den_measure_0 qbit qstate;
-          W_cstate := tm_update cstate cbit false;
-          W_prob := prob * prob0;
+          B_num_clbits := nc;
+          B_qstate := den_measure_0 qbit qstate;
+          B_cstate := tm_update cstate cbit false;
+          B_prob := prob * prob0;
         |} ::
         (Execute_measure_instr qbit cbit t)).
         nra.
       * refine ({|
-          W_num_clbits := nc;
-          W_qstate := den_measure_1 qbit qstate;
-          W_cstate := tm_update cstate cbit true;
-          W_prob := prob * prob1;
+          B_num_clbits := nc;
+          B_qstate := den_measure_1 qbit qstate;
+          B_cstate := tm_update cstate cbit true;
+          B_prob := prob * prob1;
         |} ::
         (Execute_measure_instr qbit cbit t)).
         nra.
@@ -255,54 +255,54 @@ Proof.
   + exact (Execute_measure_instr qbit cbit t).  (* nop *)
 Defined.
 
-Fixpoint Execute_reset_instr (target: nat) (worlds: ManyWorld): ManyWorld.
+Fixpoint Execute_reset_instr (target: nat) (branches: ProgramState): ProgramState.
 Proof.
-  destruct worlds as [|[nc qstate cstate prob Hp] t].
+  destruct branches as [|[nc qstate cstate prob Hp] t].
   - exact [].
   - destruct (lt_dec target nq).
     + exact ({|
-        W_num_clbits := nc;
-        W_qstate := den_reset target qstate;
-        W_cstate := cstate;
-        W_prob := prob;
-        W_prob_valid := Hp;
+        B_num_clbits := nc;
+        B_qstate := den_reset target qstate;
+        B_cstate := cstate;
+        B_prob := prob;
+        B_prob_valid := Hp;
       |} :: (Execute_reset_instr target t)).
     + exact ({|
-        W_num_clbits := nc;
-        W_qstate := qstate;
-        W_cstate := cstate;
-        W_prob := prob;
-        W_prob_valid := Hp;
+        B_num_clbits := nc;
+        B_qstate := qstate;
+        B_cstate := cstate;
+        B_prob := prob;
+        B_prob_valid := Hp;
       |} :: (Execute_reset_instr target t)).  (* nop *)
 Defined.
 
-Fixpoint Execute_suppl (ir: nat) (instr: Instruction) (worlds: ManyWorld): ManyWorld :=
+Fixpoint Execute_suppl (ir: nat) (instr: Instruction) (branches: ProgramState): ProgramState :=
   match ir with
-  | O => worlds
+  | O => branches
   | S ir' => (
     match instr with
-    | NopInstr                            => worlds
-    | RotateInstr theta phi lambda target => Execute_rotate_instr theta phi lambda target worlds
-    | CnotInstr control target            => Execute_cnot_instr control target worlds
-    | SwapInstr q1 q2                     => Execute_swap_instr q1 q2 worlds
-    | MeasureInstr qbit cbit              => Merge_manyworld (Execute_measure_instr qbit cbit worlds)
-    | SeqInstr i1 i2                      => Execute_suppl ir' i2 (Execute_suppl ir' i1 worlds)
+    | NopInstr                            => branches
+    | RotateInstr theta phi lambda target => Execute_rotate_instr theta phi lambda target branches
+    | CnotInstr control target            => Execute_cnot_instr control target branches
+    | SwapInstr q1 q2                     => Execute_swap_instr q1 q2 branches
+    | MeasureInstr qbit cbit              => Merge_program_state (Execute_measure_instr qbit cbit branches)
+    | SeqInstr i1 i2                      => Execute_suppl ir' i2 (Execute_suppl ir' i1 branches)
     | IfInstr cbit cond subinstr          => (
-        concat (map (fun w =>
-          if (eqb (W_cstate w cbit) cond)
-          then Execute_suppl ir' subinstr [w]
-          else [w]) worlds)
+        concat (map (fun b =>
+          if (eqb (B_cstate b cbit) cond)
+          then Execute_suppl ir' subinstr [b]
+          else [b]) branches)
     )
-    | ResetInstr target                   => Execute_reset_instr target worlds
+    | ResetInstr target                   => Execute_reset_instr target branches
     end
   )
   end.
 
-Definition Execute (program: InlinedProgram): ManyWorld :=
+Definition Execute (program: InlinedProgram): ProgramState :=
   Execute_suppl
     (IP_num_subinstrs program)
     (IP_instrs program)
-    (ManyWorld_init nq (IP_num_cbits program)).
+    (ProgramState_init nq (IP_num_cbits program)).
 
 Fixpoint Cstate_to_binary_little_endian (n: nat) (cstate: total_map bool) (acc: nat): nat := match n with
   | O => acc
@@ -318,13 +318,13 @@ Definition Cstate_to_binary (num_cbits: nat) (cstate: total_map bool) := Cstate_
     3 -> true *)
 
 
-Fixpoint Calculate_prob (num_cbits: nat) (worlds: ManyWorld): total_map R :=
-  match worlds with
+Fixpoint Calculate_prob (num_cbits: nat) (branches: ProgramState): total_map R :=
+  match branches with
   | [] => tm_empty R0
-  | w :: t =>
+  | b :: t =>
     let prev := Calculate_prob num_cbits t in
-    let key := Cstate_to_binary num_cbits (W_cstate w) in
-    tm_update prev key (prev key + W_prob w)%R
+    let key := Cstate_to_binary num_cbits (B_cstate b) in
+    tm_update prev key (prev key + B_prob b)%R
   end.
 
 Definition Execute_and_calculate_prob (program: InlinedProgram): total_map R :=
@@ -334,12 +334,12 @@ Definition Execute_and_calculate_prob (program: InlinedProgram): total_map R :=
 (* Proof about quantum states =================================================================== *)
 
 Lemma Execute_rotate_instr_quantum_state_density:
-  forall (theta phi lambda: R) (target: nat) (worlds: ManyWorld),
-  Forall qstate_valid worlds ->
-  Forall qstate_valid (Execute_rotate_instr theta phi lambda target worlds).
+  forall (theta phi lambda: R) (target: nat) (branches: ProgramState),
+  Forall qstate_valid branches ->
+  Forall qstate_valid (Execute_rotate_instr theta phi lambda target branches).
 Proof.
   intros.
-  induction worlds.
+  induction branches.
   - apply H.
   - destruct a.
     apply Forall_cons_iff in H.
@@ -351,20 +351,20 @@ Proof.
       apply mat_single_unitary.
       apply mat_rot_unitary.
       assumption.
-      apply IHworlds.
+      apply IHbranches.
       apply Ht.
     + apply Forall_cons; simpl.
       apply H.
-      apply IHworlds.
+      apply IHbranches.
       apply Ht.
 Qed.
 
 Lemma Execute_cnot_instr_quantum_state_density:
-  forall (control target: nat) (worlds: ManyWorld),
-  Forall qstate_valid worlds -> Forall qstate_valid (Execute_cnot_instr control target worlds).
+  forall (control target: nat) (branches: ProgramState),
+  Forall qstate_valid branches -> Forall qstate_valid (Execute_cnot_instr control target branches).
 Proof.
   intros.
-  induction worlds.
+  induction branches.
   - apply H.
   - destruct a.
     apply Forall_cons_iff in H.
@@ -376,20 +376,20 @@ Proof.
       apply den_valid_uop.
       apply mat_cnot_unitary.
       assumption.
-      apply IHworlds.
+      apply IHbranches.
       apply Ht. }
       all: apply Forall_cons.
       all: simpl; try apply H.
-      all: apply IHworlds.
+      all: apply IHbranches.
       all: apply Ht.
 Qed.
 
 Lemma Execute_swap_instr_quantum_state_density:
-  forall (q1 q2: nat) (worlds: ManyWorld),
-  Forall qstate_valid worlds -> Forall qstate_valid (Execute_swap_instr q1 q2 worlds).
+  forall (q1 q2: nat) (branches: ProgramState),
+  Forall qstate_valid branches -> Forall qstate_valid (Execute_swap_instr q1 q2 branches).
 Proof.
   intros.
-  induction worlds.
+  induction branches.
   - apply H.
   - destruct a.
     apply Forall_cons_iff in H.
@@ -401,20 +401,20 @@ Proof.
       apply den_valid_uop.
       apply mat_swap_unitary.
       assumption.
-      apply IHworlds.
+      apply IHbranches.
       apply Ht. }
       all: apply Forall_cons.
       all: simpl; try apply H.
-      all: apply IHworlds.
+      all: apply IHbranches.
       all: apply Ht.
 Qed.
 
 Lemma Execute_measure_instr_quantum_state_density:
-  forall (qbit cbit: nat) (worlds: ManyWorld),
-  Forall qstate_valid worlds -> Forall qstate_valid (Execute_measure_instr qbit cbit worlds).
+  forall (qbit cbit: nat) (branches: ProgramState),
+  Forall qstate_valid branches -> Forall qstate_valid (Execute_measure_instr qbit cbit branches).
 Proof.
   intros.
-  induction worlds.
+  induction branches.
   - apply H.
   - destruct a.
     apply Forall_cons_iff in H.
@@ -422,8 +422,8 @@ Proof.
     simpl in *.
     destruct (lt_dec qbit nq).
     + destruct
-      (Rgt_dec (com_real (den_prob_0 qbit W_qstate0)) 0),
-      (Rgt_dec (com_real (den_prob_1 qbit W_qstate0)) 0).
+      (Rgt_dec (com_real (den_prob_0 qbit B_qstate0)) 0),
+      (Rgt_dec (com_real (den_prob_1 qbit B_qstate0)) 0).
       all: try repeat apply Forall_cons; simpl.
       all: unfold den_measure_0, den_measure_1 in *.
       all: try apply den_valid_measure.
@@ -433,18 +433,18 @@ Proof.
       all: unfold com_real in *.
       all: try apply com_proj_neq_fst.
       all: unfold NTC, INR; simpl; try lra.
-      all: apply IHworlds.
+      all: apply IHbranches.
       all: apply Ht.
-    + apply IHworlds.
+    + apply IHbranches.
       apply Ht.
 Qed.
 
 Lemma Execute_reset_instr_quantum_state_density:
-  forall (target: nat) (worlds: ManyWorld),
-  Forall qstate_valid worlds -> Forall qstate_valid (Execute_reset_instr target worlds).
+  forall (target: nat) (branches: ProgramState),
+  Forall qstate_valid branches -> Forall qstate_valid (Execute_reset_instr target branches).
 Proof.
   intros.
-  induction worlds.
+  induction branches.
   - simpl.
     apply H.
   - destruct a.
@@ -455,15 +455,15 @@ Proof.
     + apply Forall_cons.
       apply den_valid_reset.
       apply H.
-      apply IHworlds.
+      apply IHbranches.
       apply Ht.
     + apply Forall_cons.
       apply H.
-      apply IHworlds.
+      apply IHbranches.
       apply Ht.
 Qed.
 
-Lemma Execute_suppl_empty_world: forall (ir: nat) (instr: Instruction),
+Lemma Execute_suppl_empty_branch: forall (ir: nat) (instr: Instruction),
   Execute_suppl ir instr [] = [].
 Proof.
   induction ir, instr.
@@ -473,10 +473,10 @@ Proof.
   reflexivity.
 Qed.
 
-Lemma Execute_suppl_nop: forall (ir: nat) (worlds: ManyWorld),
-  Execute_suppl ir NopInstr worlds = worlds.
+Lemma Execute_suppl_nop: forall (ir: nat) (branches: ProgramState),
+  Execute_suppl ir NopInstr branches = branches.
 Proof.
-  destruct ir, worlds.
+  destruct ir, branches.
   all: reflexivity.
 Qed.
 
@@ -486,8 +486,8 @@ Arguments Execute_swap_instr _ _ _ : simpl never.
 Arguments Execute_measure_instr _ _ _ : simpl never.
 
 Lemma Execute_suppl_quantum_state_density:
-  forall (ir: nat) (instr: Instruction) (worlds: ManyWorld),
-  Forall qstate_valid worlds -> Forall qstate_valid (Execute_suppl ir instr worlds).
+  forall (ir: nat) (instr: Instruction) (branches: ProgramState),
+  Forall qstate_valid branches -> Forall qstate_valid (Execute_suppl ir instr branches).
 Proof.
   intros ir instr.
   revert ir.
@@ -498,21 +498,21 @@ Proof.
   - apply Execute_rotate_instr_quantum_state_density; apply H.
   - apply Execute_cnot_instr_quantum_state_density; apply H.
   - apply Execute_swap_instr_quantum_state_density; apply H.
-  - apply Merge_manyworld_qstate_valid.
+  - apply Merge_program_state_qstate_valid.
     apply Execute_measure_instr_quantum_state_density; apply H.
   - apply IHinstr2; apply IHinstr1; apply H.
   - apply Forall_concat.
     apply Forall_map.
-    induction worlds.
+    induction branches.
     + apply Forall_nil.
     + apply Forall_cons.
-      * destruct (eqb (W_cstate a n) b).
+      * destruct (eqb (B_cstate a n) b).
         apply IHinstr.
         all: apply Forall_cons_iff in H.
         all: destruct H.
         all: apply Forall_cons.
         all: try apply H; try apply Forall_nil.
-      * apply IHworlds.
+      * apply IHbranches.
         apply Forall_cons_iff in H.
         destruct H.
         apply H0.
@@ -528,7 +528,7 @@ Proof.
   intros.
   unfold Execute.
   apply Execute_suppl_quantum_state_density.
-  unfold ManyWorld_init.
+  unfold ProgramState_init.
   apply Forall_cons.
   apply den_valid_init.
   apply Forall_nil.
